somerefactoring and exploratory code

src/named/STLC.v
@@ -9,6 +9,7 @@ Set Bullet Behavior "Strict Subproofs".
 From Ltac2 Require Import Ltac2.
 Set Default Proof Mode "Classic".
 From Utils Require Import Utils.
+From Named Require Import Exp.
 From Named Require Import IExp IRule ICore Subst Tactics.
 Require Import String.
 
@@ -259,3 +260,115 @@ Instance elab_stlc_inst : Elaborated stlc :=
   elaboration := elab_stlc;
   elab_pf := elab_stlc_pf;
   }.
+
+(* Some starter code for an STLC-specific partial recognizer
+
+TODO: do I want to try this approach?
+Fixpoint unfold_stlc_subst_list (subst_list : list (Exp.exp * Exp.exp * Exp.exp))  (e : Exp.exp) : Exp.exp :=
+  match subst_list with
+  | [::] => e
+  | (g,G',G)::sl => unfold_stlc_subst_list sl (Exp.con "ty_subst" [:: e; g; G'; G])
+  end.
+
+Lemma unfold_var_injective sl1 sl2 x1 x2
+  : (unfold_stlc_subst_list sl1 (Exp.var x1) == unfold_stlc_subst_list sl2 (Exp.var x2))
+    = (sl1 == sl2) && (x1 == x2).
+Proof.
+  revert sl2; induction sl1; intro sl2; destruct sl2; ltac1:(break); simpl; auto.
+  admit.
+  admit.
+  Search foldl.
+Admitted.
+
+Fixpoint hnf_stlc_ty (subst_list : list (Exp.exp * Exp.exp * Exp.exp))  (e : Exp.exp) : Exp.exp :=
+  match e with
+  | (Exp.con "->" args) => Exp.con "->" (map (hnf_stlc_ty subst_list) args)
+  | (Exp.con "ty_subst" [:: Exp.con "->" [:: B; A; G1']; g; G'; G]) =>
+    let hnf := hnf_stlc_ty ((g,G',G)::subst_list) in
+    Exp.con "->" [:: hnf B; hnf A; G]
+  | _ => unfold_stlc_subst_list subst_list e
+  end.
+
+Definition stlc_type_eq t1 t2 :=
+  (hnf_stlc_ty [::] t1) == (hnf_stlc_ty [::] t2).
+
+(*
+Lemma hnf_stlc_ty_con n s sb : exists n' s', hnf_stlc_ty sb (Exp.con n s) = Exp.con n' s'.
+Admitted.
+*)
+
+Lemma stlc_type_eq_constr_inv n s x
+  : ~~ (stlc_type_eq (Exp.con n s) (Exp.var x)).
+Proof using .
+  ltac1:(apply /negP).
+  unfold stlc_type_eq.
+  ltac1:(move /eqP).
+  repeat (simpl; ltac1:(case_match;try by inversion)).
+Qed.
+
+Lemma stlc_type_eq_sym a b
+  : (stlc_type_eq a b) = stlc_type_eq b a.
+Proof using .
+  apply eq_sym.
+Qed.
+
+Lemma stlc_type_eq_recognizes c e1 e2 G
+ : Core.wf_term (strip_args elab_stlc) c e1 (Exp.srt "ty" [:: G]) ->
+   Core.wf_term (strip_args elab_stlc) c e2 (Exp.srt "ty" [:: G]) ->
+   stlc_type_eq e1 e2 ->
+   Core.le_term (strip_args elab_stlc) c (Exp.srt "ty" [:: G]) e1 e2.
+Proof.
+  unfold stlc_type_eq.
+  generalize (@nil (Exp.exp *Exp.exp*Exp.exp)).
+  revert e2.
+  induction e1; intro e2; destruct e2.
+  {
+    intros l _ _.
+    intro stlceq.
+    cbn in stlceq.
+    simpl in stlceq.
+    rewrite !unfold_var_injective in stlceq.
+    ltac1:(break).
+    ltac1:(move: stlceq=> /eqP => ->).
+    reflexivity.
+  }    
+  {
+    intros sl _ _.
+    ltac1:(move /negPn).
+    admit.
+  }    
+  { admit. }  
+  {
+    intros wf1 wf2.
+    unfold stlc_type_eq.
+    match! goal with
+      [|- is_true(?a == ?b) -> _]=>
+      remember $a as l_hnf;
+        remember $b as r_hnf
+    end.
+    ltac1:(case neq: (n=="ty_subst"%string)).
+    {
+      ltac1:(move: neq => /eqP neq).
+      rewrite neq in Heql_hnf.
+      simpl in Heql_hnf.
+      rewrite neq in wf1.
+      
+      
+    issue: ty_substs
+    repeat (simpl; ltac1:(case_match)).
+  unfold stlc_type_eq in ty_eq.
+  rewrite !hnf_stlc_ty_con in ty_eq.
+  simpl in ty_eq.
+  {
+    destruct n0; try (inversion ty_eq).
+  intro wft; induction wft.
+  {
+    
+
+Fixpoint elab_lam_term (e : exp) (t : Exp.sort) : option Exp.exp :=
+  match e, t with
+  | con "lambda" [:: e], scon "el" [:: ty; G] =>
+    match simpl_stlc_ty
+  | _,_ => None
+  end.
+*)
